# 草稿

简化了动力学方程的形式：

$$
x'' = -p x_{n-1} - d x'_{n-1}, \qquad T \in [n,n+1),n \in \mathbb{N}.
$$  

对于如下线性系统：

$$
\dot{\vec{y}} = \mathcal{A} \vec{y} + \mathcal{B} \left. \vec{y} \right |_{t=(n-1)\tau},\qquad t\in[n\tau, (n+1)\tau),n \in \mathbb{N},
$$

可求解常微分方程得到：

$$
\begin{aligned}
    \left. \vec{y} \right |_{t=(n+1)\tau} &= \exp{(\mathcal{A} \tau)} \left. \vec{y} \right |_{t=n\tau} + \int_{0}^{\tau} \exp{(\mathcal{A} t_0)} dt_0 \mathcal{B} \left. \vec{y} \right |_{t = (n - 1) \tau} \\
    \left. \vec{y} \right |_{t=(n+1)\tau} &= {}^{0}A \left. \vec{y} \right |_{t=n\tau} + {}^{0}B \left. \vec{y} \right |_{t = (n - 1) \tau} \\
    \vec{y}_{n+1} &= {}^{0}A \vec{y}_{n} + {}^{0}B \vec{y}_{n-1} \\
    \Rightarrow \begin{pmatrix}
        \vec{y}_{n+1} \\ \vec{y}_{n}
    \end{pmatrix} &= \begin{bmatrix}
        {}^{0}A & {}^{0}B \\
        I & \mathbf{0}
    \end{bmatrix} \begin{pmatrix}
        \vec{y}_{n} \\ \vec{y}_{n-1}
    \end{pmatrix}.
\end{aligned}
$$

定义

$$
\vec{\Theta}_{n} = \begin{pmatrix}
    x_{n+1} \\ x'_{n+1} \\ x_{n} \\ x'_{n}
\end{pmatrix}.
$$

离散系统的演化规律为

$$
\vec{\Theta}_{n+1} = {}^{1}A \vec{\Theta}_{n}, \qquad n \in \mathbb{N}.
$$

其中，

$$
{}^{1}A = \begin{bmatrix}
    {}^{0}A & {}^{0}B \\
    I & \mathbf{0}
\end{bmatrix} =
\begin{bmatrix}
    1 & 1 & -\frac{p}{2} & -\frac{d}{2} \\
    0 & 1 & -p & -d \\
    1 & 0 & 0 & 0 \\
    0 & 1 & 0 & 0
\end{bmatrix}.
$$

可得$\vec{\theta}_{n} = (x_{n}, x'_{n})^{\top}$的表达式为：

$$
\begin{aligned}
    \vec{\theta}_{n} =
    \begin{pmatrix}
        x_{n} \\ x'_{n}
    \end{pmatrix} &=
    \begin{bmatrix}
        \mathbf{0} & I
    \end{bmatrix} \begin{pmatrix}
        x_{n+1} \\ x'_{n+1} \\ x_{n} \\ x'_{n}
    \end{pmatrix} \\
    &= \begin{bmatrix}
        \mathbf{0} & I
    \end{bmatrix} \bigg( {}^{1}A \bigg)^{n} \vec{\Theta}_{0}.
\end{aligned}
$$

在$T \in [0,1)$时，根据动力学方程：

$$
x'' = - p x_{0} - d x'_{0},
$$

可计算得到

$$
\vec{\theta}_{1} = \bigg( {}^{0}A + {}^{0}B \bigg) \vec{\theta}_{0.}
$$

因此，对于$T \in \mathbb{N}$，有

$$
\begin{aligned}
    \vec{\theta}_{T} = \vec{\theta}_{n} &= \begin{bmatrix}
        \mathbf{0} & I
    \end{bmatrix} \bigg( {}^{1}A \bigg)^{n} \vec{\Theta}_{0} \\
    &= \begin{bmatrix}
        \mathbf{0} & I
    \end{bmatrix} \bigg( {}^{1}A \bigg)^{n} \begin{bmatrix}
        \bigg( {}^{0}A + {}^{0}B \bigg) \vec{\theta}_{0} \\ \vec{\theta}_{0}
    \end{bmatrix} \\
    &= \underbrace{\begin{bmatrix}
        \mathbf{0} & I
    \end{bmatrix} \bigg( {}^{1}A \bigg)^{n} \begin{bmatrix}
        {}^{0}A + {}^{0}B \\ I
    \end{bmatrix}}_{\psi_{1} \left(n, \vec{p}, \vec{d} \right)} \vec{\theta}_{0}
\end{aligned}
$$
